Added intrinsics (subborrow and addcarry)

lib/c/libintvector.h
@@ -5,6 +5,7 @@
 #include <wmmintrin.h>
 #include <smmintrin.h>
 #include <immintrin.h>
+#include <x86intrin.h>
 
 typedef __m128i Lib_IntVector_Intrinsics_vec128;
 
@@ -342,6 +343,13 @@ typedef __m256i Lib_IntVector_Intrinsics_vec256;
   (_mm256_permute2x128_si256(x1, x2, 0x31)) 
 
 #define Lib_IntVector_Intrinsics_bit_mask64(x) -((x) & 1)
+
+#define Lib_IntVector_Intrinsics_add_carry_u64(x1, x2, x3, x4) \
+  (_addcarry_u64(x1, x2, x3, (long long unsigned int *)x4))
+
+#define Lib_IntVector_Intrinsics_sub_borrow_u64(x1, x2, x3, x4) \
+  (_subborrow_u64(x1, x3, x2, (long long unsigned int *)x4))
+
 
 
 #endif
