lib/Lib.IntVector.Intrinsics.fsti
@@ -325,3 +325,21 @@ noextract
 val vec256_smul32: vec256 -> uint32 -> vec256
 
 noextract val bit_mask64: uint64 -> uint64
+
+open FStar.Mul
+noextract
+val add_carry_u64: cin: uint64 -> x: uint64 -> y: uint64 -> r: lbuffer uint64 (size 1) -> 
+  Stack uint64 
+    (requires fun h -> live h r)
+    (ensures fun h0 c h1 -> modifies1 r h0 h1 /\ uint_v c <= 2 /\
+      (
+	let r = Seq.index (as_seq h1 r) 0 in 
+	uint_v r + uint_v c * pow2 64 == uint_v x + uint_v y + uint_v cin)
+    )
+
+noextract
+val sub_borrow_u64: cin: uint64{uint_v cin <= 1} -> x: uint64 -> y: uint64 -> r: lbuffer uint64 (size 1) -> 
+  Stack uint64
+    (requires fun h -> live h r)
+    (ensures fun h0 c h1 -> modifies1 r h0 h1 /\ 
+      (let r = Seq.index (as_seq h1 r) 0 in v r - v c * pow2 64 == v x - v y - v cin))
